examples/dynamic_isolation/Proof.v
@@ -491,12 +491,10 @@ Tactic Notation "destruct_vars" := destruct_vars_with auto.
     Definition mem_do_step_trans_input__spec :=
       @Mem_Common.do_step_trans_input__spec Memory.private_params
                                           External.ext
-                                          EnclaveParams.params
                                           Memory.rule_name_t
                                           Memory.rules
                                           Memory.schedule
                                           Memory.private_external_state_t
-                                          Memory.initial_private_external_state
                                           Memory.external_update_function.
     Definition mem_do_step__spec :=
       @Mem_Common.do_step__spec Memory.private_params
@@ -909,7 +907,6 @@ Tactic Notation "destruct_vars" := destruct_vars_with auto.
           rewrite_solve.
       Qed.
 
-
       Theorem step_rel_decoupled_step__trace :
         forall (initial_dram: dram_t) (n: nat)
           (st: state) (tr: trace) (step_ios : list mod_step_io),
@@ -1154,31 +1151,42 @@ Tactic Notation "destruct_vars" := destruct_vars_with auto.
         let machine1_log := (mem1_log ++ sm1_log ++ core1_log)%log in
         (machine0_log, machine1_log).
 
-      Definition core0_function_of_decoupled_io (st: core0_spec_state_t) (ios: list Core_Common.step_io) : Prop :=
+      Definition core0_function_of_decoupled_io__state (st: core0_spec_state_t) (ios: list Core_Common.step_io) : Prop :=
         st = fst (fst (core0_do_steps__spec ios)).
 
-      Definition core1_function_of_decoupled_io (st: core1_spec_state_t) (ios: list Core_Common.step_io) : Prop :=
+      Definition core1_function_of_decoupled_io__state (st: core1_spec_state_t) (ios: list Core_Common.step_io) : Prop :=
         st = fst (fst (core1_do_steps__spec ios)).
 
-      Definition sm_function_of_decoupled_io (st: SM_Common.spec_state_t) (ios: list SM_Common.step_io) : Prop :=
+      Definition sm_function_of_decoupled_io__state (st: SM_Common.spec_state_t) (ios: list SM_Common.step_io) : Prop :=
         st = fst (fst (Impl.System.SM.do_steps__spec ios)).
 
-      Definition mem_function_of_decoupled_io
+      Definition mem_function_of_decoupled_io__state
                  (initial_dram: dram_t) (st: mem_spec_state_t) (ios: list Mem_Common.ghost_io) : Prop :=
         st = fst (fst (mem_do_steps__spec initial_dram ios)).
 
       Definition state_function_of_decoupled_ios
                  (initial_dram: dram_t) (st: state) (step_ios: list mod_step_io) : Prop :=
-        core0_function_of_decoupled_io st.(state_core0) (map step_io_core0 step_ios) /\
-        core1_function_of_decoupled_io st.(state_core1) (map step_io_core1 step_ios) /\
-        sm_function_of_decoupled_io st.(state_sm) ((map fst (map step_io_sm step_ios))) /\
-        mem_function_of_decoupled_io initial_dram st.(state_mem) (map step_io_mem step_ios).
+        core0_function_of_decoupled_io__state st.(state_core0) (map step_io_core0 step_ios) /\
+        core1_function_of_decoupled_io__state st.(state_core1) (map step_io_core1 step_ios) /\
+        sm_function_of_decoupled_io__state st.(state_sm) ((map fst (map step_io_sm step_ios))) /\
+        mem_function_of_decoupled_io__state initial_dram st.(state_mem) (map step_io_mem step_ios).
 
-      Ltac unfold_decoupled_ios :=
-        consider @core0_function_of_decoupled_io;
-        consider @core1_function_of_decoupled_io;
-        consider @sm_function_of_decoupled_io;
-        consider @mem_function_of_decoupled_io.
+      Ltac unfold_decoupled_ios__state :=
+        consider @core0_function_of_decoupled_io__state;
+        consider @core1_function_of_decoupled_io__state;
+        consider @sm_function_of_decoupled_io__state;
+        consider @mem_function_of_decoupled_io__state.
+
+      Ltac unfold_core0_steps :=
+        consider core0_do_steps__spec;
+        consider core0_do_step_trans_input__spec.
+      Ltac unfold_core1_steps :=
+        consider core1_do_steps__spec;
+        consider core1_do_step_trans_input__spec.
+      Ltac unfold_sm_steps :=
+        consider Impl.System.SM.do_steps__spec.
+      Ltac unfold_mem_steps :=
+        consider mem_do_steps__spec.
 
       Lemma step_state_function_of_decoupled_ios :
         forall initial_dram st ios st' t io,
@@ -1187,28 +1195,28 @@ Tactic Notation "destruct_vars" := destruct_vars_with auto.
         state_function_of_decoupled_ios initial_dram st' (ios ++ [io]).
       Proof.
         intros *; intros Hdec Hstep.
-        consider state_function_of_decoupled_ios; unfold_decoupled_ios; propositional.
+        consider state_function_of_decoupled_ios; unfold_decoupled_ios__state; propositional.
         repeat rewrite map_app.
         consider do_step_with_metadata.
         consider compute_mod_outputs.
         consider compute_state.
         repeat (destruct_matches_in_hyp Hstep; simplify_tuples; subst).
         intuition; simpl.
-        - consider core0_do_steps__spec.
-          rewrite Core_Common.do_steps__spec_app.
+        - unfold_core0_steps.
+          rewrite Core_Common.do_steps__spec_app__state.
           simpl; rewrite_solve.
-        - consider core1_do_steps__spec.
-          rewrite Core_Common.do_steps__spec_app.
+        - unfold_core1_steps.
+          rewrite Core_Common.do_steps__spec_app__state.
           simpl; rewrite_solve.
-        - consider Impl.System.SM.do_steps__spec.
-          rewrite SM_Common.do_steps__spec_app.
+        - unfold_sm_steps.
+          rewrite SM_Common.do_steps__spec_app__state.
           simpl; rewrite_solve.
-        - consider mem_do_steps__spec.
-          rewrite Mem_Common.do_steps__spec_app.
+        - unfold_mem_steps.
+          rewrite Mem_Common.do_steps__spec_app__state.
           simpl; rewrite_solve.
       Qed.
 
-      Theorem step_rel_decoupled_step :
+      Theorem step_rel_decoupled_step__state :
         forall (initial_dram: dram_t) (n: nat)
           (st: state) (tr: trace) (step_ios : list mod_step_io),
           step_n_with_metadata initial_dram n = (st, tr, step_ios) ->
@@ -1216,11 +1224,108 @@ Tactic Notation "destruct_vars" := destruct_vars_with auto.
       Proof.
         induction n.
         - simpl; intuition; simplify_tuples; subst; auto;
-            consider state_function_of_decoupled_ios; unfold_decoupled_ios; auto.
+            consider state_function_of_decoupled_ios; unfold_decoupled_ios__state; auto.
         - intros; simpl in *.
           repeat destruct_matches_in_hyp H; simplify_tuples; subst.
           specialize IHn with (1 := eq_refl); propositional.
           eapply step_state_function_of_decoupled_ios; eauto.
+      Qed.
+
+      Definition core0_function_of_decoupled_io__trace
+                 (tr: list (Log Core0.R ContextEnv)) (ios: list Core_Common.step_io) : Prop :=
+        tr = snd (fst (core0_do_steps__spec ios)).
+
+      Definition core1_function_of_decoupled_io__trace
+                 (tr: list (Log Core1.R ContextEnv)) (ios: list Core_Common.step_io) : Prop :=
+        tr = snd (fst (core1_do_steps__spec ios)).
+
+      Definition sm_function_of_decoupled_io__trace
+                 (tr: list (SM_Common.spec_output_t)) (ios: list SM_Common.step_io) : Prop :=
+        tr = snd (fst (Impl.System.SM.do_steps__spec ios)).
+
+      Definition mem_function_of_decoupled_io__trace
+                 (initial_dram: dram_t) (tr: list (Log Memory.R ContextEnv * Log Memory.R ContextEnv))
+                 (ios: list Mem_Common.ghost_io) : Prop :=
+        tr = snd (fst (mem_do_steps__spec initial_dram ios)).
+
+      Definition trace_function_of_decoupled_ios
+                 (initial_dram: dram_t) (tr: trace) (step_ios: list mod_step_io) : Prop :=
+        core0_function_of_decoupled_io__trace (map output_core0 tr) (map step_io_core0 step_ios) /\
+        core1_function_of_decoupled_io__trace (map output_core1 tr) (map step_io_core1 step_ios) /\
+        sm_function_of_decoupled_io__trace (map output_sm tr) (map fst (map step_io_sm step_ios)) /\
+        mem_function_of_decoupled_io__trace initial_dram (map output_mem tr) (map step_io_mem step_ios).
+
+      Ltac unfold_decoupled_ios__trace :=
+        consider @core0_function_of_decoupled_io__trace;
+        consider @core1_function_of_decoupled_io__trace;
+        consider @sm_function_of_decoupled_io__trace;
+        consider @mem_function_of_decoupled_io__trace.
+
+      Lemma step_trace_function_of_decoupled_ios :
+        forall initial_dram st ios st' tr t io,
+        state_function_of_decoupled_ios initial_dram st ios ->
+        trace_function_of_decoupled_ios initial_dram tr ios ->
+        do_step_with_metadata st = (st', t, io) ->
+        trace_function_of_decoupled_ios initial_dram (tr ++ [t]) (ios ++ [io]).
+      Proof.
+        intros *; intros Hst Htr Hstep.
+        consider trace_function_of_decoupled_ios; unfold_decoupled_ios__trace; propositional.
+        repeat rewrite map_app.
+        consider do_step_with_metadata.
+        consider compute_mod_outputs.
+        repeat (destruct_matches_in_hyp Hstep; simplify_tuples; subst).
+        consider state_function_of_decoupled_ios; propositional; unfold_decoupled_ios__state.
+        intuition; simpl.
+        - rewrite Htr0.
+          consider do_core0.
+          unfold_core0_steps.
+          destruct_matches_in_hyp Heqp.
+          simplify_tuples; subst.
+          repeat rewrite<-Core_Common.do_steps__spec_app__trace.
+          simpl Core_Common.step_input.
+          rewrite<-Hst0.
+          rewrite_solve.
+        - rewrite Htr2.
+          consider do_core1.
+          unfold_core1_steps.
+          destruct_matches_in_hyp Heqp0.
+          simplify_tuples; subst.
+          rewrite<-Core_Common.do_steps__spec_app__trace.
+          simpl Core_Common.step_input.
+          rewrite<-Hst2.
+          rewrite_solve.
+        - rewrite Htr1.
+          consider do_sm.
+          unfold_sm_steps.
+          destruct_matches_in_hyp Heqp1.
+          simplify_tuples; subst.
+          rewrite Hst1 in Heqp3.
+          rewrite<-SM_Common.do_steps__spec_app__trace.
+          simpl SM_Common.step_input.
+          rewrite_solve.
+        - rewrite Htr4.
+          consider do_mem.
+          unfold_mem_steps.
+          simplify_tuples; subst.
+          rewrite<-Mem_Common.do_steps__spec_app__trace.
+          simpl Mem_Common.step_input.
+          rewrite_solve.
+      Qed.
+
+      Theorem step_rel_decoupled_step__trace :
+        forall (initial_dram: dram_t) (n: nat)
+          (st: state) (tr: trace) (step_ios : list mod_step_io),
+          step_n_with_metadata initial_dram n = (st, tr, step_ios) ->
+          trace_function_of_decoupled_ios initial_dram tr step_ios.
+      Proof.
+        induction n.
+        - simpl; intuition; simplify_tuples; subst; auto;
+            consider trace_function_of_decoupled_ios; unfold_decoupled_ios__trace; auto.
+        - intros; simpl in *.
+          repeat destruct_matches_in_hyp H; simplify_tuples; subst.
+          specialize IHn with (1 := eq_refl); propositional.
+          eapply step_trace_function_of_decoupled_ios; eauto.
+          eapply step_rel_decoupled_step__state; eauto.
       Qed.
 
     End HelperLemmas.
